Semantics/Dynamic/Bool.v
@@ -1,6 +1,10 @@
 From Coq Require Import ssreflect.
 
+From ExtensibleCompiler.Semantics.Static Require Import Bool.
+
 From ExtensibleCompiler.Syntax.Terms Require Import Bool.
+
+From ExtensibleCompiler.Syntax.Types Require Import BoolType.
 
 From ExtensibleCompiler.Theory Require Import Algebra.
 From ExtensibleCompiler.Theory Require Import Eval.
@@ -38,31 +42,46 @@ Inductive Eval__Bool {L V}
   | BoolValue : forall b, Eval__Bool Eval_E (boolean b, boolean b)
 .
 
+Inductive WellTyped__Bool
+          {T E}
+          `{FunctorLaws T} `{FunctorLaws E}
+          `{! T supports BoolType}
+          `{! E supports Bool}
+          (WT : TypedExpr T E -> Prop) : TypedExpr T E -> Prop :=
+| WellTyped__boolean : forall t e b,
+    proj1_sig e = boolean__F b ->
+    proj1_sig t = boolType ->
+    WellTyped__Bool WT {| type := t; expr := e; |}.
+
 Definition SoundnessStatement__Bool
-           {L LT V}
-           `{FunctorLaws L} `{FunctorLaws LT} `{FunctorLaws V}
-           `{! L supports Bool}
-           (WT : (TypedValue V LT -> Prop) -> TypedValue V LT -> Prop)
-           `{Eval_L   : forall {T}, ProgramAlgebra Eval   L T (EvalResult   V)}
-           `{TypeOf_L : forall {T}, ProgramAlgebra TypeOf L T (TypeOfResult LT)}
-           (recEval   : UniversalPropertyF L -> EvalResult   V)
-           (recTypeOf : UniversalPropertyF L -> TypeOfResult LT)
+           {T E V}
+           `{FunctorLaws T} `{FunctorLaws E} `{FunctorLaws V}
+           `{! E supports Bool}
+           (WT : (TypedExpr T V -> Prop) -> TypedExpr T V -> Prop)
+           `{Eval__E   : forall {R}, ProgramAlgebra Eval   E R (EvalResult   V)}
+           `{TypeOf__E : forall {R}, ProgramAlgebra TypeOf E R (TypeOfResult T)}
+           (recEval   : UniversalPropertyF E -> EvalResult   V)
+           (recTypeOf : UniversalPropertyF E -> TypeOfResult T)
   :=
     (SoundnessStatement__EvalAlgebra WT
-                                   (evalL   := fun _ => programAlgebra' Eval_L)
-                                   (typeOfL := fun _ => programAlgebra' TypeOf_L)
+                                   (eval__E   := fun _ => programAlgebra' Eval__E)
+                                   (typeOf__F := fun _ => programAlgebra' TypeOf__E)
                                    recEval recTypeOf
     ).
 
 Global Instance EvalSoundness__Bool
-       {L LT V}
-       `{FunctorLaws L} `{FunctorLaws LT} `{FunctorLaws V}
-       `{! L supports Bool}
-       (WT : (TypedValue V LT -> Prop) -> TypedValue V LT -> Prop)
-       `{Eval_L   : forall {T}, ProgramAlgebra Eval   L T (EvalResult   V)}
-       `{TypeOf_L : forall {T}, ProgramAlgebra TypeOf L T (TypeOfResult LT)}
-       (recEval   : UniversalPropertyF L -> EvalResult   V)
-       (recTypeOf : UniversalPropertyF L -> TypeOfResult LT)
+       {T E V}
+       `{FunctorLaws T} `{FunctorLaws E} `{FunctorLaws V}
+       `{! E supports Bool} `{! WellFormedSubFunctor Bool E}
+       `{! T supports BoolType}
+       `{! V supports Bool}
+       (WT : (TypedExpr T V -> Prop) -> TypedExpr T V -> Prop)
+       `{Eval__E   : forall {R}, ProgramAlgebra Eval   E R (EvalResult   V)}
+       `{! forall {R}, WellFormedProgramAlgebra EvalAlgebra__Bool Eval__E (T := R)}
+       `{TypeOf__E : forall {R}, ProgramAlgebra TypeOf E R (TypeOfResult T)}
+       `{! forall {R}, WellFormedProgramAlgebra TypeOf__Bool TypeOf__E (T := R)}
+       (recEval   : UniversalPropertyF E -> EvalResult   V)
+       (recTypeOf : UniversalPropertyF E -> TypeOfResult T)
   : ProofAlgebra Bool (sig (UniversalPropertyP2 (SoundnessStatement__Bool WT recEval recTypeOf))).
 Proof.
   constructor.
@@ -73,8 +92,20 @@ Proof.
     apply conj; apply (proj2_sig (boolean b)).
   }
   {
-    move => Gamma IH T TY.
+    move => Gamma.
     rewrite / boolean__F / boolean / inject /=.
+    rewrite unwrap__UP'_wrap__F /=.
+    rewrite fmapFusion / Extras.compose /=.
+    rewrite wellFormedSubFunctor => //=.
+    rewrite / programAlgebra'.
+    rewrite wellFormedProgramAlgebra.
+    rewrite wellFormedProgramAlgebra.
+    move => IH tau.
+    rewrite / programAlgebra.
+    rewrite / EvalAlgebra__Bool / eval__Bool.
+    rewrite / TypeOf__Bool / typeOf__Bool.
+    move => [] <-.
+    rewrite / WellTyped.
 
     admit.
   }
